Complete ZKboo completeness proof

code/Commitment.ec
@@ -11,22 +11,70 @@ type randomness.
 
 op dm : {message distr | is_lossless dm} as dm_ll.
 op dr : {randomness distr | is_lossless dr} as dr_ll.
+op dkey : {(secret_key * public_key) distr | is_lossless dkey} as dkey_ll.
+
+op verify (pk : public_key, m : message, c : commitment, d : randomness): bool.
 
 module type Protocol = {
-  proc key_gen() : secret_key * public_key
+  (* proc * key_gen() : secret_key * public_key *)
   proc commit(sk : secret_key, m : message) : commitment * randomness
-  proc verify(pk : public_key, m : message, c : commitment, d : randomness) : bool
 }.
 
 module Correctness(P : Protocol) = {
   proc main(m : message) : bool = {
     var sk, pk, c, d, b;
-    (sk, pk) = P.key_gen();
+    (sk, pk) <$ dkey;
     (c, d)   = P.commit(sk, m);
-    b        = P.verify(pk, m, c, d);
+    b = verify pk m c d;
     return b;
   }
+
+  proc key_fixed(m : message, sk : secret_key, pk : public_key) : bool = {
+    var c, d, b;
+    (c, d)   = P.commit(sk, m);
+    b = verify pk m c d;
+    return b;
+  }
+
+  proc intermediate(m : message) = {
+    var sk, pk, b;
+    (sk, pk) <$ dkey;
+    b = key_fixed(m, sk, pk);
+    return b;
+
+  }
 }.
+
+lemma intermediate (Com <: Protocol) m' &m:
+    Pr[Correctness(Com).main(m') @ &m : res] =
+    Pr[Correctness(Com).intermediate(m') @ &m : res].
+proof.
+  byequiv=>//. proc.
+  inline *. sim.
+qed.
+
+lemma key_fixed_correct (Com <: Protocol) m' &m:
+    (forall sk' pk', phoare[Correctness(Com).key_fixed : sk = sk' /\ pk = pk' /\ (sk', pk') \in dkey ==> res] = 1%r)
+    => Pr[Correctness(Com).main(m') @ &m : res] = 1%r.
+proof.
+  move => H.
+  have -> := (intermediate Com m' &m).
+  byphoare(: m = m' ==> )=>//.
+  proc.
+  seq 1 : (#pre /\ exists sk' pk', sk = sk' /\ pk = pk' /\ (sk', pk') \in dkey).
+  auto. auto. progress.
+  apply dkey_ll.
+  smt().
+  elim * => sk' pk'.
+  have H' := H sk' pk'.
+  call H'.
+  skip; progress.
+  hoare.
+  auto. progress. smt().
+  progress.
+qed.
+
+
 
 module type HidingAdv = {
   (* proc * means that this operation initializes the modules state *)
@@ -39,7 +87,7 @@ module type HidingAdv = {
 module HidingGame(P : Protocol, A : HidingAdv) = {
   proc main() = {
     var sk, pk, m0, m1, b, b', c, r;
-    (sk, pk) = P.key_gen();
+    (sk, pk) <$ dkey;
     (m0, m1) = A.get();
     b <$ DBool.dbool;
     if (b) {
@@ -59,10 +107,10 @@ module type BindingAdv = {
 module BindingGame(P : Protocol, B : BindingAdv) = {
   proc main() = {
   var sk, pk, c, m, m', r, r', v, v';
-    (sk, pk) = P.key_gen();
+    (sk, pk) <$ dkey;
     (c, m, m', r, r') = B.bind(sk, pk);
-    v = P.verify(pk, m, c, r);
-    v' = P.verify(pk, m', c, r');
+    v = verify pk m c r;
+    v' = verify pk m' c r';
     return (v /\ v') /\ (m <> m');
   }
 }.
