code/ZKBoo.ec
@@ -1,5 +1,5 @@
 (* Formalization of ZKBoo Sigma-protocol *)
-require import AllCore Distr List DInterval Decompose.
+require import AllCore Distr List DInterval DList Decompose.
 require (****) SigmaProtocols.
 require import Commitment.
 (** Ignore: This is now the preferred setup but is not yet the default **)
@@ -8,26 +8,465 @@ pragma -oldip. pragma +implicits.
 (* TODO index into view *)
 (* TODO constuct random tape *)
 (* pred valid_view w1 w2 k1 k2 = forall j, w1 = phi_decomp *)
+op valid_view w = w /\ true.
+
+clone import Commitment as Commit with
+  type message <- view.
+
+print Com.
 
 type statement  = (circuit * int).
 type witness    = int.
-type message    = output * output * output * commitment * commitment * commitment.
+type message    = output * output * output * Commit.commitment * Commit.commitment * Commit.commitment.
 type challenge  = int.
-type response   = secret_key * secret_key.
+type response   = public_key * ((view * randomness) * (view * randomness)).
 
-op R_DL h w     = let (c, h') = h in (h' = eval_circuit c [w]).
+axiom challenge_size (c : challenge) : 0 < c <= 3.
+
+op R_DL h w     = let (c, y) = h in (y = eval_circuit c [w]).
 
 clone import SigmaProtocols as Sigma with
-  type SigmaProtocols.statement <- statement,
-  type SigmaProtocols.witness <- witness,
-  type SigmaProtocols.message <- message,
-  type SigmaProtocols.challenge <- challenge,
-  type SigmaProtocols.response <- response,
+  type statement <- statement,
+  type witness <- witness,
+  type message <- message,
+  type challenge <- challenge,
+  type response <- response,
 
-  op SigmaProtocols.R = R_DL,
-  op SigmaProtocols.dchallenge = [1..3]
+  op R = R_DL,
+  op dchallenge = [1..3]
   proof *.
-  realize SigmaProtocols.dchallenge_llfuni.
+  realize dchallenge_llfuni.
       (* TODO: by [dt_ll, dt_funi] *)
-      split. apply dinter_ll. trivial. apply dinter_uni. qed.
-export SigmaProtocols.
+      split. apply dinter_ll. trivial. apply is_full_funiform.
+      rewrite /is_full.
+      progress.
+      case (0 < x <= 3).
+      smt.
+      move=> H.
+      have : 0 < x <= 3. apply challenge_size.
+      smt().
+      apply dinter_uni.
+  qed.
+export Sigma.
+
+module ZKBoo(Com : Protocol) : SProtocol = {
+  var pk : public_key
+  var r1, r2, r3 : randomness
+  var w1, w2, w3 : view
+  proc gen() : statement * witness = {
+    return (([], 0),0);
+  }
+  proc init(h : statement, w : witness) = {
+    var x1,x2,x3,y,c,c1,c2,c3,sk,y1,y2,y3;
+    (c, y) = h;
+    (sk, pk) <$ Commit.dkey;
+    (x1, x2, x3) = Phi.share(w);
+    (w1, w2, w3) = Phi.compute(c, [x1], [x2], [x3]);
+    (c1, r1) = Com.commit(sk, w1);
+    (c2, r2) = Com.commit(sk, w2);
+    (c3, r3) = Com.commit(sk, w3);
+    y1 = Phi.output(w1);
+    y2 = Phi.output(w2);
+    y3 = Phi.output(w3);
+
+    return (y1,y2,y3,c1,c2,c3);
+  }
+
+  proc response(h : statement, w : witness, m : message, e : challenge) = {
+    var ret;
+    if (e = 1) {
+      ret = ((w1, r1), (w2, r2));
+    } else {
+      if (e = 2) {
+        ret = ((w2, r2), (w3, r3));
+      } else {
+        ret = ((w3, r3), (w1, r1));
+      }
+    }
+    return (pk, ret);
+  }
+
+  proc valid_output_share(y : output, w : view) : bool = {
+    var share;
+    share = Phi.output(w);
+    return y = share;
+  }
+
+  (* proc valid_view(w w' : view, k k' : random_tape) = { *)
+  (*   while (w <> []) { *)
+  (*     s = head w; *)
+  (*     s' = head w'; *)
+  (*     r = head k; *)
+  (*     r' = head k'; *)
+
+  (*     (* TODO *) *)
+
+  (*     w = behead w; *)
+  (*     w' = behead w'; *)
+  (*     k = behead k; *)
+  (*     k' = behead k'; *)
+  (*   } *)
+  (* } *)
+
+  proc verify(h : statement, m : message, e : challenge, z : response) = {
+    var c, pk, open, y1, y2, y3, c1, c2, c3, y, y', valid_com1, valid_com2;
+    var valid_share1, valid_share2;
+    var w1', w2', w3', r1', r2', r3';
+    (pk, open) = z;
+    (y1, y2, y3, c1, c2, c3) = m;
+    (c, y) = h;
+
+    if (e = 1) {
+      (w1', r1') = fst open;
+      (w2', r2') = snd open;
+      valid_com1 = Commit.verify pk w1' c1 r1';
+      valid_com2 = Commit.verify pk w2' c2 r2';
+      valid_share1 = valid_output_share(y1, w1');
+      valid_share2 = valid_output_share(y2, w2');
+    } else {
+      if (e = 2) {
+        (w2', r2') = fst open;
+        (w3', r3') = snd open;
+        valid_com1 = Commit.verify pk w2' c2 r2';
+        valid_com2 = Commit.verify pk w3' c3 r3';
+        valid_share1 = valid_output_share(y2, w2');
+        valid_share2 = valid_output_share(y3, w3');
+      } else {
+        (w3', r3') = fst open;
+        (w1', r1') = snd open;
+        valid_com1 = Commit.verify pk w3' c3 r3';
+        valid_com2 = Commit.verify pk w1' c1 r1';
+        valid_share1 = valid_output_share(y3, w3');
+        valid_share2 = valid_output_share(y1, w1');
+
+      }
+    }
+
+    y' = Phi.reconstruct(y1, y2, y3);
+
+    return y' = y /\ valid_com1 /\ valid_com2 /\ valid_share1 /\ valid_share2;
+
+  }
+
+  proc witness_extractor(h : statement, m : message, e e' : challenge, z z' : response) = {
+    return 0;
+  }
+
+  proc simulator(h : statement, e : challenge) = {
+    var c, y, views, sk, pk, a, z;
+    var w1, w2, y1, y2, y3;
+    var c1, c2, c3, r1, r2, r3;
+    (c, y) = h;
+    (views, y3) = Privacy.ideal(y, c, e);
+    (w1, w2) = views;
+    w3 <$ dlist dinput (size w1);
+    y1 = Phi.output(w1);
+    y2 = Phi.output(w2);
+
+    (sk, pk) <$ Commit.dkey;
+    (c1, r1) = Com.commit(sk, w1);
+    (c2, r2) = Com.commit(sk, w2);
+    (c3, r3) = Com.commit(sk, w3);
+    a = (y1, y2, y3, c1, c2, c3);
+    z = (pk, ((w1, r1), (w2, r2)));
+
+    return (a, z);
+  }
+
+}.
+
+section Protocol.
+
+declare module Com : Commit.Protocol{ZKBoo}.
+
+(* Assume security of Com *)
+(* axiom Com_correct &m a : Pr[Correctness(Com).main(a) @ &m : res] = 1%r. *)
+
+axiom Com_correct :
+    phoare[Correctness(Com).key_fixed : (sk, pk) \in Commit.dkey ==> res] = 1%r.
+axiom Com_hiding &m (A <: HidingAdv):
+  Pr[HidingGame(Com, A).main() @ &m : res] = 1%r.
+axiom Com_binding &m (A <: BindingAdv):
+  Pr[BindingGame(Com, A).main() @ &m : res] = 1%r.
+axiom commit_ll : islossless Com.commit.
+
+
+local module Intermediate = {
+  module ComCorrectness = Correctness(Com)
+  proc valid_output_share(y : output, w : view) : bool = {
+    var share;
+    share = Phi.output(w);
+    return y = share;
+  }
+
+  proc main(h : statement, w : witness, e : challenge) = {
+    var x1,x2,x3,sk,pk,y1,y2,y3,y';
+    var c,y,w1,w2,w3,valid_com1,valid_com2,valid_share1,valid_share2;
+    (c, y) = h;
+    (x1, x2, x3) = Phi.share(w);
+    (w1, w2, w3) = Phi.compute(c, [x1], [x2], [x3]);
+    y1 = Phi.output(w1);
+    y2 = Phi.output(w2);
+    y3 = Phi.output(w3);
+    (sk, pk) <$ Commit.dkey;
+    if (e = 1) {
+      valid_com1 = ComCorrectness.key_fixed(w1, sk, pk);
+      valid_com2 = ComCorrectness.key_fixed(w2, sk, pk);
+      Com.commit(sk, w3);
+      valid_share1 = valid_output_share(y1, w1);
+      valid_share2 = valid_output_share(y2, w2);
+    } else {
+      if (e = 2) {
+        Com.commit(sk, w1);
+        valid_com1 = ComCorrectness.key_fixed(w2, sk, pk);
+        valid_com2 = ComCorrectness.key_fixed(w3, sk, pk);
+        valid_share1 = valid_output_share(y2, w2);
+        valid_share2 = valid_output_share(y3, w3);
+      } else {
+        valid_com2 = ComCorrectness.key_fixed(w1, sk, pk);
+        Com.commit(sk, w2);
+        valid_com1 = ComCorrectness.key_fixed(w3, sk, pk);
+        valid_share1 = valid_output_share(y3, w3);
+        valid_share2 = valid_output_share(y1, w1);
+      }
+    }
+
+    y' = Phi.reconstruct(y1,y2,y3);
+    return y' = y /\ valid_com1 /\ valid_com2 /\ valid_share1 /\ valid_share2;
+  }
+}.
+
+local lemma inter_completeness h' w' e' &m:
+    R h' w' =>
+    Pr[Intermediate.main(h', w', e') @ &m : res] = 1%r.
+proof.
+  rewrite /R /R_DL. rewrite pairS.
+  progress.
+  byphoare(: (h = h' /\ w = w' /\ e = e') ==>)=>//; last first. smt().
+  proc.
+  case (e' = 1).
+    rcondt 8. auto. do ? call(:true); auto.
+    inline Intermediate.valid_output_share Phi.output Phi.reconstruct Phi.share.
+    sp. wp.
+    call commit_ll.
+    call Com_correct.
+    call Com_correct.
+    auto.
+    call (compute_circuit_correct h'.`1 [w']).
+    auto; progress.
+    apply dinput_ll.
+    smt().
+    apply Commit.dkey_ll.
+    smt().
+    have : (result.`1, result.`2, result.`3) = result by smt().
+    rewrite /eval_circuit in H.
+    have Hlast := last_nth 0.
+    smt().
+  case (e' = 2).
+    rcondf 8. auto. do ? call(:true); auto.
+    rcondt 8. auto. do ? call(:true); auto.
+    inline Intermediate.valid_output_share Phi.output Phi.reconstruct Phi.share.
+    sp. wp.
+    call Com_correct.
+    call Com_correct.
+    call commit_ll.
+    auto.
+    call (compute_circuit_correct h'.`1 [w']).
+    auto; progress.
+    apply dinput_ll.
+    smt().
+    apply Commit.dkey_ll.
+    smt().
+    have : (result.`1, result.`2, result.`3) = result by smt().
+    rewrite /eval_circuit in H.
+    have Hlast := last_nth 0.
+  (* case (e' = 2) *)
+    smt().
+    rcondf 8. auto. do ? call(:true); auto.
+    rcondf 8. auto. do ? call(:true); auto.
+    inline Intermediate.valid_output_share Phi.output Phi.reconstruct Phi.share.
+    sp. wp.
+    call Com_correct.
+    call commit_ll.
+    call Com_correct.
+    auto.
+    call (compute_circuit_correct h'.`1 [w']).
+    auto; progress.
+    apply dinput_ll.
+    smt().
+    apply Commit.dkey_ll.
+    smt().
+    have : (result.`1, result.`2, result.`3) = result by smt().
+    rewrite /eval_circuit in H.
+    have Hlast := last_nth 0.
+    smt().
+qed.
+
+local equiv inter_equiv :
+    Sigma.Completeness(ZKBoo(Com)).special ~ Intermediate.main :
+    ={h, w, e, glob Com} /\ R h{1} w{1} ==> ={res}.
+proof.
+  proc.
+  inline ZKBoo(Com).init ZKBoo(Com).response ZKBoo(Com).verify.
+  sp.
+  case (e{1} = 1).
+  rcondt{1} 15. progress.
+    auto; do ? call (:true); auto.
+  rcondt{2} 7. progress.
+    auto; do ? call (:true); auto.
+  rcondt{1} 24. progress.
+    auto; do ? call (:true); auto.
+  inline Phi.reconstruct.
+  inline ZKBoo(Com).valid_output_share Intermediate.valid_output_share.
+  inline Intermediate.ComCorrectness.key_fixed.
+  swap{2} [11..12] 5.
+  swap{2} [15..18] 1.
+  swap{2} [3..5] 10.
+  swap{2} 2 1.
+  swap{1} 1 1.
+  auto.
+  sim.
+  auto.
+  call (:true); auto.
+  call (:true); auto.
+  call (:true); auto.
+  call (:true); auto.
+  call (:true); auto.
+  call (:true); auto.
+  call (:true). sim.
+  auto.
+  call (:true). sim.
+  skip; progress.
+  case (e{1} = 2).
+  rcondf{1} 15. progress.
+    auto; do ? call (:true); auto.
+  rcondt{1} 15. progress.
+    auto; do ? call (:true); auto.
+  rcondf{2} 7. progress.
+    auto; do ? call (:true); auto.
+  rcondt{2} 7. progress.
+    auto; do ? call (:true); auto.
+  rcondf{1} 24. progress.
+    auto; do ? call (:true); auto.
+  rcondt{1} 24. progress.
+    auto; do ? call (:true); auto.
+  inline Phi.reconstruct.
+  inline ZKBoo(Com).valid_output_share Intermediate.valid_output_share.
+  inline Intermediate.ComCorrectness.key_fixed.
+  auto. sim. auto.
+  swap{2} [12..13] 4.
+  wp.
+  swap{2} [3..5] 10.
+  swap{2} 2 1.
+  swap{1} 1 1.
+  call (:true); auto.
+  call (:true); auto.
+  call (:true); auto.
+  call (:true); auto.
+  call (:true); auto.
+  call (:true); auto.
+  call (:true). sim.
+  auto.
+  call (:true). sim.
+  skip; progress.
+
+  (* case e = 3 *)
+  rcondf{1} 15. progress.
+    auto; do ? call (:true); auto.
+  rcondf{1} 15. progress.
+    auto; do ? call (:true); auto.
+  rcondf{2} 7. progress.
+    auto; do ? call (:true); auto.
+  rcondf{2} 7. progress.
+    auto; do ? call (:true); auto.
+  rcondf{1} 24. progress.
+    auto; do ? call (:true); auto.
+  rcondf{1} 24. progress.
+    auto; do ? call (:true); auto.
+  inline Phi.reconstruct.
+  inline ZKBoo(Com).valid_output_share Intermediate.valid_output_share.
+  inline Intermediate.ComCorrectness.key_fixed.
+  auto. sim. auto.
+  swap{2} [11..12] 5. wp.
+  swap{2} [3..5] 10.
+  swap{2} 2 1.
+  swap{1} 1 1.
+  call (:true); auto.
+  call (:true); auto.
+  call (:true); auto.
+  call (:true); auto.
+  call (:true); auto.
+  call (:true); auto.
+  call (:true). sim.
+  auto.
+  call (:true). sim.
+  skip; progress.
+qed.
+
+lemma zkboo_completeness h' w' e' &m:
+    R h' w' =>
+    Pr[Sigma.Completeness(ZKBoo(Com)).special(h', w', e') @ &m : res] = 1%r.
+proof.
+  move=> rel.
+  have -> : Pr[Completeness(ZKBoo(Com)).special(h', w', e') @ &m : res] =
+            Pr[Intermediate.main(h', w', e') @ &m : res].
+  - byequiv inter_equiv=>//.
+  by have := inter_completeness h' w' e' &m rel.
+qed.
+
+
+(* idea: reduce to Phi.main; Com.correctness *)
+lemma zkboo_complete &m h' w' e':
+    R h' w' =>
+    Pr[Sigma.Completeness(ZKBoo(Com)).special(h', w', e') @ &m : res] = 1%r.
+proof.
+  rewrite /R /R_DL.
+  move=> rel.
+  byphoare(: h = h' /\ w = w' /\ e = e' ==> _)=>//.
+  proc.
+  inline Completeness(ZKBoo(Com)).special.
+  inline ZKBoo(Com).init.
+  swap 4 2.
+  swap [6..9] 3.
+  inline Phi.share. sp.
+  seq 3 : (#pre /\ exists (x1' x2' x3' : input), x1' = x10 /\ x2' = x20 /\ x3' = x30 /\ x1' + x2' + x3' = w'); last first; last first.
+    - hoare. auto. progress. smt().
+    - progress.
+    - auto. auto. progress.
+      apply dinput_ll. smt().
+  sp. elim *. progress.
+  have Hcompute := compute_circuit_correct (fst h') [x1'] [x2'] [x3'] [w'] (eval_circuit_aux (fst h') [w']) _.
+   - smt().
+  inline ZKBoo(Com).response.
+  inline ZKBoo(Com).verify.
+  case (e' = 1).
+    auto. rcondt 23.
+    auto.
+    call (:true).
+    call (:true).
+    call (:true).
+    call (:true).
+    call (:true). auto.
+    call (:true). auto.
+    call (:true). auto.
+    call (:true). auto.
+    auto.
+  rcondt 14.
+    auto.
+    call (:true).
+    call (:true).
+    call (:true).
+    call (:true).
+    call (:true); auto.
+    call (:true); auto.
+    call (:true); auto.
+    call (:true); auto.
+  inline Phi.reconstruct. auto.
+  inline ZKBoo(Com).valid_output_share Phi.output.
+  auto.
+  sp.
+  swap 1 2.
+
+
+
+end section Protocol.
